theories/logrel/logrel.v
@@ -16,11 +16,6 @@ Section logrel.
   Definition pages_in_trans (trans: gmap Word transaction) : gset PID :=
     map_fold (λ (k:Addr) v acc, v.1.1.2 ∪ acc) (∅: gset PID) trans.
 
-  Definition set_of_addr (ps:gset PID) := (set_fold (λ p (acc:gset Addr), list_to_set (addr_of_page p) ∪ acc) ∅ ps).
-
-  (* TODO *)
-  Definition memory_pages (ps :gset PID): iProp Σ:=
-    ∃ mem, (⌜dom (gset Addr) mem = set_of_addr ps⌝ ∗ [∗ map] k ↦ v ∈ mem, k ->a v)%I.
   Definition pgt (ps: gset PID) q (vo: VMID) (be: bool) : iProp Σ :=
     [∗ set] p ∈ ps, p -@{q}O> vo ∗ p -@{q}E> be.
 
@@ -82,8 +77,8 @@ Section logrel.
      the memory is the memory of pages associated with a transaction and i has or may have access to. *)
   Definition trans_memory_in_trans (trans : gmap Word transaction) :=
     filter (λ kv, (kv.2.1.1.1.1.1 = i ∧ ¬(kv.2.2 = true ∧ kv.2.1.2 = Lending)) ∨ kv.2.1.1.1.2 = i) trans.
-  Definition memory_transferred (trans : gmap Word transaction) :=
-    memory_pages (pages_in_trans (trans_memory_in_trans trans)).
+  Definition memory_transferred (trans : gmap Word transaction) (mem: mem) :=
+   memory_pages (pages_in_trans (trans_memory_in_trans trans)) mem.
 
   Definition VMProp_unknown p_tx p_rx trans : iProp Σ:=
     ∃ ps_na' ps_acc' (trans' : gmap Word transaction) hpool' rx_state ,
@@ -103,13 +98,13 @@ Section logrel.
                transaction_pagetable_entries_transferred trans' ∗
                retrieval_entries trans' ∗
                (* memory *)
-               memory_transferred trans' ∗
+               (∃ mem_trans, memory_transferred trans' mem_trans)∗
                R0 @@ V0 ->r encode_hvc_func(Run) ∗ R1 @@ V0 ->r encode_vmid(i) ∗
                (* status of RX *)
                RX_state@ i := rx_state ∗
                (* RX *)
                (rx_page i p_rx) ∗
-               memory_pages {[p_rx]} ∗
+               (∃ mem_rx, memory_page p_rx) ∗
                (* Implications: these implications relate [trans], the transactions at the beginning of the proof, and
                 [trans'], those at the point of switching to i. These assumptions are (I believe) necessary to prove FTLR.
                 Moreover, they are provable because of that fact that i as the invoker is the only vm can manipulate
@@ -121,8 +116,8 @@ Section logrel.
                 the proofs to the users of LR. *)
                (transaction_pagetable_entries_owned trans -∗ transaction_pagetable_entries_owned trans') ∗
                (pagetable_entries_excl_owned i ps_oea -∗ pagetable_entries_excl_owned i ps_oea') ∗
-               (memory_pages ps_oea ∗ memory_transferred trans' -∗
-                memory_pages (ps_acc' ∖ {[p_rx;p_tx]} ∪ ps_macc_trans')) ∗
+               ((∃ mem_oea, memory_pages ps_oea) ∗ (∃ mem_trans, memory_transferred trans' mem_trans) -∗
+                ∃ mem_all, memory_pages (ps_acc' ∖ {[p_rx;p_tx]} ∪ ps_macc_trans') mem_all) ∗
                (* if i yielding, we give following resources back to pvm *)
                VMProp V0
                       ((∃ ps_na'' ps_acc'' trans'' hpool'',
@@ -136,7 +131,7 @@ Section logrel.
                            transaction_pagetable_entries_transferred trans'' ∗
                            retrieval_entries trans'' ∗
                            (* memory *)
-                           memory_pages ps_macc_trans'' ∗
+                           (∃ mem_macc_trans, memory_pages ps_macc_trans'' mem_macc_trans) ∗
                            R0 @@ V0 ->r encode_hvc_func(Yield) ∗ R1 @@ V0 ->r encode_vmid(i) ∗
                            (* status of RX *)
                            (match rx_state with
@@ -144,7 +139,7 @@ Section logrel.
                               | Some _ => RX_state@ i := None ∨ RX_state@i := rx_state
                             end) ∗
                            (* RX *)
-                           rx_page i p_rx ∗ memory_pages {[p_rx]})
+                           rx_page i p_rx ∗ ∃ mem_rx, memory_page p_rx mem_rx)
                            (* no scheduling, we finish the proof *)
                            ∨ False) (1/2)%Qp
              .
@@ -163,8 +158,8 @@ Section logrel.
       ⌜{[p_tx;p_rx]} ⊆ ps_acc⌝ ∗
       pagetable_entries_excl_owned i ps_oea ∗
       transaction_pagetable_entries_owned trans ∗
-      memory_pages ps_oea ∗
-       VMProp i (VMProp_unknown p_tx p_rx trans) (1/2)%Qp
+      (∃ mem_oea, memory_pages ps_oea) ∗
+      VMProp i (VMProp_unknown p_tx p_rx trans) (1/2)%Qp
     )%I.
 
   (* Things we haven't really considerred:
