theories/rules/mem_share.v
@@ -1,0 +1,54 @@
+From machine_program_logic.program_logic Require Import weakestpre.
+From HypVeri Require Import lifting rules.rules_base machine_extra.
+From HypVeri.algebra Require Import base mem reg pagetable mailbox trans base_extra.
+From HypVeri.lang Require Import lang_extra reg_extra mem_extra pagetable_extra trans_extra.
+
+Section mem_share.
+
+Context `{hypparams: HypervisorParameters}.
+Context `{vmG: !gen_VMG Σ}.
+
+Lemma hvc_mem_share_nz {i wi r0 r1 r2 hvcf p_tx sacc } ai j mem_tx sh (spsd: gset PID) :
+  (* len is the length of the msg *)
+  let len := (Z.of_nat (finz.to_z r1)) in
+  (* the decoding of wi is correct *)
+  decode_instruction wi = Some(Hvc) ->
+  (* the decoding of R0 is a FFA mem send *)
+  decode_hvc_func r0 = Some(hvcf) ->
+  hvcf_to_tt hvcf = Some Sharing ->
+  (* caller is not the receiver *)
+  i ≠ j ->
+  (* the descriptor, in list Word *)
+  (* des = serialized_transaction_descriptor i j W0 l (elements spsd) W0 -> *)
+  (* the whole descriptor resides in the TX page *)
+  (len < page_size)%Z ->
+  (* there is at least one free handle in the hpool *)
+  sh ≠ ∅ ->
+  {SS{{ ▷(PC @@ i ->r ai) ∗
+      ▷ ai ->a wi ∗
+  (* VM i owns pages in spsd *)
+      ▷ ([∗ set] p ∈ spsd, p -@O> i) ∗
+  (* pages in spsed are exclusive to VM i *)
+      ▷ (i -@A> sacc) ∗
+      (* and the page which the instruction is in is not being shared, i.e. (tpa ai) ∉ spsd *)
+      ▷ (R0 @@ i ->r r0) ∗
+      ▷ (R1 @@ i ->r r1) ∗
+      ▷ (R2 @@i ->r r2) ∗
+      ▷ (fresh_handles 1 sh) ∗
+      ▷ TX@ i := p_tx ∗
+      ▷ mem_region des p_tx
+       }}}
+   ExecI @ i {{{ RET (false,ExecI) ;
+                 PC @@ i ->r (ai ^+ 1)%f ∗
+                 ai ->a wi ∗
+                 ([∗ set] p ∈ spsd, p -@O> i ) ∗
+                 i -@A> (sacc ∖ spsd) ∗
+                 R0 @@ i ->r (encode_hvc_ret_code Succ) ∗
+                 R1 @@ i ->r r1 ∗
+                 (∃ (wh: Word), ⌜wh ∈ sh⌝ ∗
+                 R2 @@ i ->r wh ∗
+                 wh ->t (i,W0,j,spsd,Sharing) ∗
+                 wh ->re false ∗
+                 fresh_handles 1 (sh∖{[wh]})) ∗
+                 TX@ i := p_tx ∗
+                 mem_region des p_tx}}}.
